improvement

FOL.v
@@ -17,78 +17,92 @@ match s with
 end.
 
 Variable formula : Type.
+Variable subst : (nat -> term) -> formula -> formula.
+Notation "[ A ] p" := (subst A p) (at level 31).
 
 Inductive f_atomic : Type -> Type :=
   | Pred : forall (P : Preds), Vector.t term (p_ar P) -> f_atomic formula
   | Bot : f_atomic formula.
+Notation "⊥" := (Bot).
 
 Definition subst_atomic (sigma : nat -> term) (s : f_atomic formula) : f_atomic formula :=
 match s with
-  | Bot => Bot
+  | ⊥ => ⊥
   | Pred P args => Pred P (Vector.map (subst_term sigma) args)
 end.
 
 Inductive f_implicative : Type -> Type :=
   | Imp : formula -> formula -> f_implicative formula.
-
-(* 
-Fixpoint subst_implicative (sigma : nat -> term) (s : formula_implicative formula) : formula_implicative formula :=
-match s with
-  | Imp p q => Imp (subst_implicative sigma p) (subst_implicative sigma q)
-end.
- *)
-
-Inductive f_universal (formula : Type) :=
-  | Univ : formula -> f_universal formula.
-(* 
-  Fixpoint subst_universal (sigma : nat -> term) (s : formula) : formula :=
-  match s with
-    | Univ p => Univ (subst_universal (fun n => sigma (S n)) p)
-  end.
- *)
-
-
 Notation "p ~> q" := (Imp p q) (at level 51, right associativity).
-Notation "! p" := (p ~> Bot) (at level 35, right associativity).
-(* 
-Definition instantiate t := subst_form (fun n => match n with 0 => t | n => Var n end).
-Definition shifted := map (subst_form (fun n => Var (S n))).
- *)
-Reserved Notation "H |- p" (at level 70).
-Implicit Types H : list formula.
-(* 
-Inductive nd H : formula -> Prop :=
-  | ndHyp p  : In p H -> H |- p
-  | ndExp p  : H |- Bot  ->  H |- p
-  | ndII p q : p::H |- q  -> H |- p ~> q
-  | ndIE p q : H |- p ~> q  ->  H |- p  -> H |- q
-  | ndUI p : shifted H |- p -> H |- Univ p
-  | ndUE t p : H |- Univ p -> H |- instantiate t p 
-where "H |- p" := (nd H p).
- *)
-Inductive deduction_atomic H : f_atomic formula -> Prop :=
-  | ndHyp p  : In p H -> H |- p
-  | ndExp p  : H |- Bot  ->  H |- p
-where "H |- p" := (deduction_atomic H p).
+(* Notation "! p" := (p ~> Bot) (at level 35, right associativity). *)
 
-Theorem weakening A B p : A |- p -> incl A B -> B |- p.
+Definition subst_implicative (sigma : nat -> term) (s : f_implicative formula) : f_implicative formula :=
+match s with
+  | p ~> q => [sigma]p ~> [sigma]q
+end.
+
+Inductive f_universal : Type -> Type :=
+  | Univ : formula -> f_universal formula.
+Notation "∀ p" := (Univ p) (at level 52).
+
+Definition subst_universal (sigma : nat -> term) (s : f_universal formula) : f_universal formula :=
+match s with
+  | ∀ p => ∀ [fun n => sigma (S n)]p
+end.
+
+Reserved Notation "A |- p" (at level 70).
+Inductive deduction (A : list formula) : formula -> Prop :=
+  | ndHyp p : In p A -> A |- p
+where "A |- p" := (deduction A p).
+
+
+Reserved Notation "A |-_atm p" (at level 70).
+Inductive deduction_atomic (A : list formula) : f_atomic formula -> Prop :=
+  | ndExp p  : A |-_atm ⊥  ->  A |-_atm p
+where "H |-_atm p" := (deduction_atomic H p).
+
+Reserved Notation "A |-_imp p" (at level 70).
+Inductive deduction_implicative (A : list formula) : formula + f_implicative formula -> Prop :=
+  | ndII p q : p::A |- q  -> A |-_imp inr (p ~> q)
+  | ndIE p q : A |-_imp inr (p ~> q)  ->  A |- p  -> A |-_imp inl q
+where "A |-_imp p" := (deduction_implicative A p).
+
+
+Definition instantiate t := subst (fun n => match n with 0 => t | n => Var n end).
+Definition shifted := map (subst (fun n => Var (S n))).
+
+Reserved Notation "A |-_unv p" (at level 70).
+Inductive deduction_universal (A : list formula) : formula + f_universal formula -> Prop :=
+  | ndUI p : shifted A |-_unv inl p -> A |-_unv inr (∀ p)
+  | ndUE t p : A |-_unv inr (∀ p) -> A |-_unv inl (instantiate t p)
+where "A |-_unv p" := (deduction_universal A p).
+
+Lemma weakening A B p : A |- p -> incl A B -> B |- p.
 Proof. induction 1; intro Hinc.
   -apply ndHyp. now apply (Hinc p).
+Qed.
+
+Lemma weakening_atm A B p : A |-_atm p -> incl A B -> B |-_atm p.
+Proof. induction 1 as [ p nd ]; intro Hinc.
   -now apply ndExp, IHnd.
-  -apply ndII. admit.
-  -apply (ndIE _ _ _ (IHnd1 Hinc) (IHnd2 Hinc)).
+Qed.
+
+Lemma weakening_imp A B p : A |-_imp p -> incl A B -> B |-_imp p.
+Proof. induction 1 as [ p q nd | p q nd ]; intro Hinc.
+  -apply ndII, (weakening (p::A)). assumption.
+   intros a [Hh | Ht]. now left. right. now apply (Hinc a).
+  -apply (ndIE _ p q). now apply IHnd. now apply (weakening A).
+Qed.
+
+Lemma weakening_unv A B p : A |-_unv p -> incl A B -> B |-_unv p.
+Proof. revert A B. induction 1 as [ Hs p nd | Hs t p nd ]; intro Hinc.
   -apply ndUI. admit.
   -now apply ndUE, IHnd.
 Admitted.
 
-Theorem double_neg_int H p : H |- p -> H |- !!p.
-Proof. induction 1; apply ndII.
-  -assert (!p :: H |- !p). {apply ndHyp. now left. }
-   assert (!p :: H |- p). {apply ndHyp. now right. }
-   apply (ndIE _ _ _ H1 H2).
-  -apply (weakening H _ ). assumption. intros p1 H1. now right.
-  -admit.
-  -admit.
-  -admit.
-  -admit.
-Admitted.
+
+(* TODO  define implicative+falsity variant to proove A|-p -> A|-(p~>⊥)~>⊥ *)
+
+Inductive f_1 : Type :=
+  | inj_atm (a : f_atomic f_1)
+  | inj_imp (i : f_implicative f_1).
